\documentclass{article}
\usepackage{amsmath}
\usepackage{amssymb}
\usepackage{hyperref}

\begin{document}
    Prove that
    \begin{equation}
        \sum_{k=0}^{t} \binom{t-k}{r} \binom{k}{s} = \binom{t+1}{r+s+1}\label{eq:identity-to-prove}
    \end{equation}

    We can see that iteration in the left-hand side of the equation~\eqref{eq:identity-to-prove} is running
    over the upper index of binomial coefficients, so let's figure out proper generating function for it.
    We know that
    \begin{equation}
        \sum_{n=0}^{\infty} \binom{n}{k} y^n = \frac{y^k}{(1-y)^{k+1}}\label{eq:generating-function-base}
    \end{equation}
    Now we keep attention to the lower index of binomial coefficient in right-hand side
    of the equation~\eqref{eq:identity-to-prove} which is $r+s+1$.
    We have to match some generating function to reach the $\sum_{n=0}^{\infty} \binom{n}{r+s+1} x^n$
    Let be generating functions
    \begin{align*}
        A_r(x) &= \sum_{l=0}^{\infty} \binom{l}{r} x^l\\
        B_s(x) &= \sum_{k=0}^{\infty} \binom{k}{s} x^k
    \end{align*}
    Now let's match our generating function
    \begin{align*}
        x A_r(x) B_s(x)
        &= x \cdot \left( \sum_{l=0}^{\infty} \binom{l}{r} x^l \right) \cdot \left( \sum_{k=0}^{\infty} \binom{k}{s} x^k \right) \\
        &= x \cdot \frac{x^r}{(1-x)^{r+1}} \cdot \frac{x^s}{(1-x)^{s+1}} = \frac{x^{r+s+1}}{(1-x)^{r+s+2}} \\
        &= \sum_{n=0}^{\infty} \binom{n}{r+s+1} x^n
    \end{align*}
    Because of the equation~\eqref{eq:generating-function-base}.
    Actually, we could simply substitute $k=r+s$ to the equation~\eqref{eq:generating-function-base} to reach desired
    generating function, anyway.

    The coefficient of $x^{t+1}$ in the $x \cdot \sum_{l=0}^{\infty} \binom{l}{r} x^l \cdot \sum_{k=0}^{\infty} \binom{k}{s} x^k$ is
    \begin{align*}
    [x^{t+1}]
        x A_r(x) B_s(x) = \sum_{k=0}^{t} a_k b_{t-k} = \sum_{k=0}^{t} \binom{t-k}{r} \binom{k}{s}
    \end{align*}
    Note that upper summation bound is $t$ while coefficient is $[z^{t+1}]$ it is because of the $x$ factor in the generating function.
    General rule for that is
    \begin{align*}
    [z^{p-q}]A(z)=[z^p]z^qA(z)
    \end{align*}
    While
    \begin{align*}
    [z^{t+1}]
        \sum_{n=0}^{\infty} \binom{n}{r+s+1} x^n = \binom{t+1}{r+s+1}
    \end{align*}
    Thus
    \begin{align*}
        \binom{t+1}{r+s+1} = \sum_{k=0}^{t} \binom{t-k}{r} \binom{k}{s}
    \end{align*}

    This approach is based on generating functions
    by \url{http://math.arizona.edu/~faris/combinatoricsweb/generate.pdf}
%    \begin{align*}
%        \sum_{l+k=t} \binom{l}{r} \binom{k}{s}
%    \end{align*}
%    Let $n = t + 1$, $\binom{t+1}{r+s+1} = \sum_{l+k=t} \binom{l}{r} \binom{k}{s} = \sum_{0 \leq k \leq t} \binom{t-k}{r} \binom{k}{s}$

\end{document}
