\begin{identity}
    Cauchy product rule of two generating functions $A(z), \; B(z)$
    \begin{align*}
        A(z) \cdot B(z) = \left( \sum_{n=0}^{\infty} a_n z^n \right) \left( \sum_{n=0}^{\infty} b_n z^n \right)
        = \sum_{n=0}^{\infty} \left( \sum_{k=0}^{n} a_k b_{n-k} \right) z^n
    \end{align*}
\end{identity}
\begin{identity}
    Cauchy product rule for $(1+z)^{r+s}$
    \begin{align*}
    (1 + z)
        ^{r+s} = \sum_{n=0}^{\infty} \left( \sum_{k=0}^{n} \binom{r}{k} \binom{s}{n-k} \right) z^n
    \end{align*}
\end{identity}
\begin{identity}
    Shift selected coefficient of generating function
    \begin{align*}
    [z^{p-q}]
        A(z)=[z^p] z^{q} A(z) \\
        [z^{p+q}] A(z)=[z^p] \frac{1}{z^{q}} A(z)
    \end{align*}
\end{identity}
\begin{identity}
    Binomial coefficient, fixed $r$
    \begin{align*}
        \binom{r}{n} = \coefficientOf{z}{n} (1+z)^r
    \end{align*}
\end{identity}
\begin{identity}
    Shifted binomial coefficient, fixed $m, r$
    \begin{align*}
        \binom{r}{m+n} &= \coefficientOf{z}{n} \frac{(1+z)^r}{z^m} \\
        \binom{r}{n-m} &= \coefficientOf{z}{n} (1+z)^r z^m \\
    \end{align*}
\end{identity}
\begin{identity}
    Binomial coefficient of multiset~\cite[eq. 8]{faris2011generating}, fixed k
    \begin{align*}
        A_k(z) = \sum_{n=0}^{\infty} \binom{n}{k} z^n = \frac{z^k}{(1-z)^{k+1}}
    \end{align*}
    Then
    \begin{align*}
        \binom{t}{k} = \coefficientOf{z}{t} \frac{z^k}{(1-z)^{k+1}}
    \end{align*}
    So that
    \begin{align*}
        \coefficientOf{z}{t} \sum_{m=0}^{\infty} \binom{m}{k} z^m = \coefficientOf{z}{t} \frac{z^k}{(1-z)^{k+1}}
    \end{align*}
\end{identity}
\begin{identity}
    Shifted Binomial coefficient of multiset, fixed k
    \begin{align*}
        \binom{t}{k+r} = \coefficientOf{z}{t} \frac{z^{k+r}}{(1-z)^{k+r+1}}
    \end{align*}
\end{identity}
\begin{identity}
    Shifted Binomial coefficient of multiset in two variables~\cite[eq. 15]{faris2011generating}
    \begin{align*}
        \sum_{n=0}^{\infty} (1 + x)^n y^n = \frac{1}{1 - (1 + x)y}
    \end{align*}
\end{identity}
\begin{identity}
    Shifted Binomial coefficient of multiset in two variables (negated)
    \begin{align*}
        \sum_{n=0}^{\infty} (1 + x)^n y^n (-1)^n = \frac{1}{1 + (1 + x)y}
    \end{align*}
\end{identity}
\begin{identity}
    Binomial coefficients row summation East-West
    \begin{align*}
        \sum_{k} \binom{r}{j-k}
        &= \sum_{k} \coefficientOf{z}{j-k}(1+z)^r
        = \coefficientOf{z}{j} \sum_{k} z^k (1+z)^r \\
        &= (1+z)^r \coefficientOf{z}{j} \sum_{k} z^k
    \end{align*}
    Because $[z^{p-q}] A(z)=[z^p] z^{q} A(z)$
\end{identity}




\clearpage
