\section{Problem 2: Concrete mathematics equation (5.22)}
\label{sec:problem-2:-concrete-mathematics-equation-(5.22)}
Use generating functions to prove that
\begin{equation}
    \sum_{k} \binom{r}{m+k} \binom{s}{n-k} = \binom{r+s}{m+n}
    \label{eq:identity-to-prove}
\end{equation}
Okay, first let's review the summation boundary such that terms are non-zero.
Summation is done over $k$ so that binomial coefficient $\binom{s}{n-k}$ fixes $k$ to be less or equal to $n$.
Rewrite the statement of the problem
\begin{equation}
    \sum_{k=0}^{n} \binom{r}{m+k} \binom{s}{n-k} = \binom{r+s}{m+n}
    \label{eq:identity-to-prove-2}
\end{equation}
Left-hand side of it reminds me sequence convolution of two generating functions.
Let be two generating functions for such left-hand side summation:
\begin{equation*}
    A_r(z); \quad B_s(z)
\end{equation*}
Multiplying those generating functions yields
\begin{align*}
    C(x) = \left(\sum_{m=0}^{\infty} a_m x^m\right) \left(\sum_{n=0}^{\infty} b_n x^n\right) = \sum_{k=0}^{\infty} \left( \sum_{m=0}^{k} a_m b_{k-m} \right) x^k
\end{align*}
Then
\begin{align*}
    A_r(z) \cdot B_s(z) = \sum_{n=0}^{\infty} \left( \sum_{k=0}^{n} a_k b_{n-k} \right) x^n
\end{align*}
We can notice the similar structure as we have in our problem~\eqref{eq:identity-to-prove-2}.
So let's find the generating function for the binomial coefficient $\binom{r+s}{m+n}$.
We know that generating function for the binomial coefficient $\binom{n}{k}$ is
\begin{align*}
(1+z)
    ^{n} = \sum_{k=0}^{\infty} \binom{n}{k} z^k
\end{align*}
If we want to have $m+k$ as lower index, then
\begin{align*}
(1+z)
    ^{r} = \sum_{k=0}^{\infty} \binom{r}{m+k} z^{m+k} \\
    (1+z)^{r} = z^m \sum_{k=0}^{\infty} \binom{r}{m+k} z^{k} \\
    \frac{(1+z)^{r}}{z^m} = \sum_{k=0}^{\infty} \binom{r}{m+k} z^{k}
\end{align*}
Thus, the coefficient of $z^n$ in $\frac{(1+z)^{r}}{z^m}$ is
\begin{align*}
[z^n]
    \frac{(1+z)^{r}}{z^m} = \binom{r}{m+n}
\end{align*}
So that our first generating function is
\begin{align*}
    A_r(z) = \frac{(1+z)^{r}}{z^m}
\end{align*}
The second generating function is
\begin{align*}
    B_s(z) = (1+z)^{s}
\end{align*}
Multiplying them
\begin{align*}
    A_r(z) \cdot B_s(z) = \frac{(1+z)^{r}}{z^m} \cdot (1+z)^{s} = \frac{(1+z)^{r+s}}{z^m}
\end{align*}
Convolution form is
\begin{align*}
    A_r(z) \cdot B_s(z) = \sum_{n=0}^{\infty} \left( \sum_{k=0}^{n} a_k b_{n-k} \right) x^n \\
    = \sum_{n=0}^{\infty} \left( \sum_{k=0}^{n} \binom{r}{m+k} \binom{s}{n-k} \right) x^n
\end{align*}
Coefficient of $z^n$ in $\frac{(1+z)^{r+s}}{z^m}$ is
\begin{align*}
[z^n]
    \frac{(1+z)^{r+s}}{z^m} = \binom{r+s}{m+n}
\end{align*}
Coefficient of $z^n$ in $\sum_{k=0}^{\infty} \left( \sum_{k=0}^{n} \binom{r}{m+k} \binom{s}{n-k} \right) x^n$ is
\begin{align*}
[z^n]
    A_r(z) \cdot B_s(z) = \sum_{k=0}^{n} \binom{r}{m+k} \binom{s}{n-k}
\end{align*}

\clearpage
