\section{Problem 3: Prove that $\sum_{k} \binom{l}{m+k} \binom{s}{n+k} = \binom{l+s}{l-m+n}$}
\label{sec:problem-3:-concrete-mathematics-equation-(5.23)}
This is from Concrete mathematics equation (5.23).
See also \url{https://math.stackexchange.com/q/4967193/463487}.
Use generating functions to prove that
\begin{equation}
    \sum_{k} \binom{l}{m+k} \binom{s}{n+k} = \binom{l+s}{l-m+n}
    \label{eq:identity-to-prove-problem-3}
\end{equation}
The first problem is that it is not clear what summation bounds should be to keep non-zero terms.
Let's reverse the coefficient $\binom{l}{m+k}$ to see exact summation bounds
\begin{align*}
    \sum_{k=0}^{l-m} \binom{l}{l-m-k} \binom{s}{n+k} = \binom{l+s}{l-m+n}
\end{align*}
So now it is clear that we are hunting for the coefficient of $z^{l-m}$ in the generating function.
Let's rearrange the sum above
\begin{align*}
    \sum_{k=0}^{(l-m)} \binom{s}{n+k} \binom{l}{(l-m)-k} = \binom{l+s}{n+(l-m)}
\end{align*}
So we can see that left-hand side of the equation above matches the convolution of two generating functions.
\begin{align*}
    A(z) \cdot B(z) = \sum_{n=0}^{\infty} \left( \sum_{k=0}^{n} a_k b_{n-k} \right) z^n
\end{align*}
having $n=l-m$ so that basically our identity is taking the coefficient of $z^{l-m}$
in the convolution of two generating functions.
Let be $n=t$ for the sake of simplicity
\begin{equation}
    \sum_{k=0}^{(l-m)} \binom{s}{t+k} \binom{l}{(l-m)-k} = \binom{l+s}{t+(l-m)}
    \label{eq:identity-to-prove-problem-3-2}
\end{equation}
So we have to match two generating functions $A_s(z), \; B_l(z)$ for
the binomial coefficients: $\binom{s}{t+k}$ and $\binom{l}{(l-m)-k}$.
So that
\begin{align*}
    A_s(z) = \frac{(1+z)^s}{z^t} \\
    B_l(z) = (1+z)^l \\
\end{align*}
So that product of them
\begin{align*}
    A_s(z) \cdot B_l(z) = \sum_{n=0}^{\infty} \left( \sum_{k=0}^{n} \binom{s}{t+k} \binom{l}{n-k} \right) z^n
    = \frac{(1+z)^s}{z^t} \cdot (1+z)^l = \frac{(1+z)^{l+s}}{z^t}
\end{align*}
Right side of the~\eqref{eq:identity-to-prove-problem-3-2} is the coefficient of
$z^{l-m}$ in $\frac{(1+z)^{l+s}}{z^t}$
\begin{align*}
[z^{l-m}]
    \frac{(1+z)^{l+s}}{z^t} = \binom{l+s}{l-m+t}
\end{align*}
Left side of the~\eqref{eq:identity-to-prove-problem-3-2} is the coefficient of $z^{l-m}$
in the convolution of two generating functions
\begin{align*}
[z^{l-m}]
    A_s(z) \cdot B_l(z) = \sum_{k=0}^{(l-m)} \binom{s}{t+k} \binom{l}{(l-m)-k}
\end{align*}
Thus,
\begin{align*}
    \sum_{k=0}^{(l-m)} \binom{s}{t+k} \binom{l}{(l-m)-k} = \binom{l+s}{l-m+t}
\end{align*}

\clearpage
