\section{Problem 6: Prove that $\sum_{k \leq n} \binom{k}{m} = \binom{n+1}{m+1}$}
\label{sec:problem-6}
This is from Concrete Mathematics equation (5.10).
Using generating function prove that
\begin{align}
    \sum_{k=0}^{n} \binom{k}{m} = \binom{n+1}{m+1}
    \label{eq:identity-to-prove-problem-6}
\end{align}
Now it is clear that we are looking for the coefficient of $z^n$ in the convolution of two generating functions.
Rewrite problem to match the Cauchy product rule
\begin{align}
    \sum_{k=0}^{n} \binom{k}{m} \binom{n-k}{j} = \binom{n+1}{m+1}
    \label{eq:problem-6-general-form}
\end{align}
Generating function for the binomial coefficient $\binom{k}{m}$ is given by
\begin{align*}
    A_m(z) = \sum_{k=0}^{\infty} \binom{k}{m} z^k = \frac{z^m}{(1-z)^{m+1}}
\end{align*}
Generating function for the binomial coefficient $\binom{n-k}{j}$ is given by
\begin{align*}
    B_j(z) = \sum_{k=0}^{\infty} \binom{k}{j} z^k = \frac{z^j}{(1-z)^{j+1}}
\end{align*}
Multiplication of them yields
\begin{align*}
    A_m(z) \cdot B_j(z)
    &= \sum_{n=0}^{\infty} \left( \sum_{k=0}^{n} \binom{k}{m} \binom{n-k}{j} \right) z^n
    = \frac{z^m}{(1-z)^{m+1}} \cdot \frac{z^j}{(1-z)^{j+1}} \\
    &= \frac{z^{m+j}}{(1-z)^{m+j+2}}
\end{align*}
Let $j=0$ then
\begin{align*}
    A_m(z) \cdot B_0(z) = \frac{z^m}{(1-z)^{m+1}} \cdot \frac{1}{(1-z)} = \frac{z^m}{(1-z)^{m+2}}
\end{align*}
Note that generating function above does not match the generating function of binomial coefficient $\binom{k}{n}$,
fixed $n$.
Multiplying by $z$ gives
\begin{align*}
    z A_m(z) \cdot B_0(z)
    &= \sum_{n=0}^{\infty} \left( \sum_{k=0}^{n} \binom{k}{m} \binom{n-k}{0} \right) z^{n+1}
    = \frac{z^m}{(1-z)^{m+1}} \cdot \frac{1}{(1-z)} \\
    = \frac{z^{m+1}}{(1-z)^{m+2}}
\end{align*}
Now it matches.
Taking the coefficient of $z^{n+1}$ yields
\begin{align*}
    [z^{n+1}] z A_m(z) \cdot B_0(z) = \binom{n+1}{m+1}
\end{align*}
Therefore, it is indeed true that
\begin{align*}
    \sum_{k=0}^{n} \binom{k}{m} = \binom{n+1}{m+1}
\end{align*}
\clearpage
