\section{Problem 7: Prove that $\sum_{k\leq m} \binom{r}{k} (-1)^k = (-1)^m \binom{r-1}{m}$}
\label{sec:problem-7}

This is from Concrete Mathematics equation (5.16).
Using generating function prove that
\begin{equation}
    \sum_{k\leq m} \binom{r}{k} (-1)^k = (-1)^m \binom{r-1}{m}
    \label{eq:problem-7}
\end{equation}
Let be $m=n$ for the sake of clarity
\begin{align*}
    \sum_{k=0}^{n} \binom{r}{k} (-1)^k = (-1)^n \binom{r-1}{n}
\end{align*}
So we are looking for the coefficient of $z^n$ in multiplication of certain generating functions $A, B$.
Rewrite the problem
\begin{align*}
    \sum_{k=0}^{n} 1 \cdot \binom{r}{r-k} (-1)^k = (-1)^n \binom{r-1}{n}
\end{align*}
So that generating function for all $1$ is $A$
\begin{align*}
    A(z) = \frac{1}{1-z}
\end{align*}
For $\binom{r}{r-k} (-1)^k$ is $B(z)$
\begin{align*}
    B_r (z) = (1-z)^r
\end{align*}
Multiplication of those generating functions yields
\begin{align*}
    A(z) \cdot B_r (z) = \frac{1}{1-z} \cdot (1-z)^r = (1-z)^{r-1}
\end{align*}
Therefore the coefficient of $z^n$ in $A(z) \cdot B_r (z) = (1-z)^{r-1}$ is
\begin{align*}
    \coefficientOf{z}{n} (1-z)^{r-1} = (-1)^n \binom{r-1}{n}
\end{align*}
Therefore, identity is true
\begin{align*}
    \sum_{k=0}^{n} \binom{r}{k} (-1)^k = (-1)^n \binom{r-1}{n}
\end{align*}



\clearpage
